\documentclass[11pt]{article}

\makeatletter
\newcommand{\skipitems}[1]{%
	\addtocounter{\@enumctr}{#1}%
}
\makeatother

\newcommand{\numpy}{{\tt numpy}}
\usepackage{amsfonts}
\usepackage{amsmath}
\usepackage{graphics}
\usepackage{amsthm,amstext,amsfonts,bm,amssymb}
\usepackage{graphicx}
\graphicspath{ {./images/} }
\usepackage{indentfirst}
\setlength{\parindent}{5ex}
\setlength{\parskip}{1em}
\usepackage[utf8x]{inputenc} 
\usepackage[russian]{babel}
\topmargin -.5in
\textheight 9in
\oddsidemargin -.25in
\evensidemargin -.25in
\textwidth 7in


\begin{document}
	
	\author{Биктимиров Данила, группа 204}
	\title{ДЗ 10}
	\date{}
	\maketitle
	
	\medskip
	
	\begin{enumerate}
		\item \begin{enumerate}
			\item Сделаем замену $w = \frac{y^2}{x}\:v = \frac{x^2}{y}$. Тогда $$2p\le w\le 2q \:\: 2r\le v \le 2s$$ $$ x=w^{\frac{1}{3}}v^{\frac{2}{3}} \:\: x=w^{\frac{2}{3}}v^{\frac{1}{3}}$$
			
			Якобиан $$\det \begin{pmatrix}
				\frac{1}{3}w^{-\frac{2}{3}}v^{\frac{2}{3}} && \frac{2}{3}w^{\frac{1}{3}}v^{-\frac{1}{3}} \\
				\frac{2}{3}w^{-\frac{1}{3}}v^{\frac{1}{3}} && \frac{1}{3}w^{\frac{2}{3}}v^{-\frac{2}{3}}
			\end{pmatrix} = \frac{1}{9}-\frac{4}{9} = -\frac{1}{3} \Rightarrow \text{ модуль якобиана } \frac{1}{3}$$
			$$ S=\int_{2p}^{2q}du\int_{2r}^{2s}\frac{1}{3}dv=\frac{4}{3}(q-p)(s-r) $$
			\item Сделаем замену $x=ar(\cos^4 \phi)\:\:y = br(\sin^4 \phi)\Rightarrow0\le\sqrt{r}\le 1,\:\: 0\le \phi \le\frac{\pi}{2}$ Якобиан $$\det \begin{pmatrix}
				a(\cos^4 \phi) && -ar\cos^3\phi\sin\phi \\
				b(\sin^4 \phi) && 4br\sin^3\phi\cos\phi \frac{1}{3}w^{\frac{2}{3}}v^{-\frac{2}{3}}
			\end{pmatrix} = 4abr\cos^3\phi\sin^3\phi$$
			$$ S=\int_{r\le1,0\le\phi\le\frac{\pi}{2}}\int 4abr\cos^3\phi\sin^3\phi dx dy=\int_{0}^{\frac{\pi}{2}}2ab\cos^3\phi\sin^3\phi\frac{ab}{6} $$
		\end{enumerate}
	\item \begin{enumerate}
		\item $z \leq x^2 + y^2, y \geq x^2, y < 1, z \geq 0$
		$$ V = \int_{-1}{1}dx\int_{x^2}{1}dy\int_{0}{x^2+y^2}dz=\int_{-1}{1}dx\int_{x^2}{1}(x^2+y^2)dy = $$ $$= \int_{-1}^{1}dx\left(x^2y+\frac{y^3}{3}\right) \mid_{x^2}^1 = \int_{-1}^{1}\left(x^2+\frac{1}{3}\right)-\left(x^4+\frac{x^6}{3}\right)dx =$$ $$ =\left(\frac{x^3}{3} + \frac{x}{3}-\frac{x^5}{5}-\frac{x^7}{21}\right)\mid_{-1}^1 =\frac{88}{105}$$
		\item Делаем $x=ar\cos \phi\:\:\: y=br\sin\phi$. Тогда $r^2-\frac{z^2}{c^2}\ge -1\:\:\:-c\sqrt{r^2+1}\le z\le c\sqrt{r^2+1}$ $$ det\begin{pmatrix}
			a\cos\phi && -ra\sin\phi && 0\\
			b\sin\phi && rb\cos\phi && 0\\
			0 && 0 && 1
		\end{pmatrix} =abr$$
		$$ V=\int_{0}^{2\pi}dy\int_{0}^{1}dr\int_{-c\sqrt{r^2+1}}^{c\sqrt{r^2+1}}abr dz  = \int_{0}^{2\pi} dy \int_{0}^{1} 2abcr\sqrt{r^2+1}dr=$$ $$ = abc\int_{0}^{2\pi}dy\int_{0}^{1} d2r \sqrt{r^2+1}=abc\int_{0}^{2\pi} dy \int_{1}^{2} \sqrt{t}dt= $$ $$ = abc\int_{0}^{2\pi} dy (\frac{\sqrt[2]{t^3}}{3}|^2_1)=\frac{4abc\pi(\sqrt{2}-1)}{3}$$
	\end{enumerate}
	\item $$\int_0^1dx\int_0^1dy\int_0^{x^2+y^2}dz$$
	$$0 \leq x \leq 1\:\:\:0 \leq y \leq 1\:\:\:0 \leq z \leq 2$$
	
	Есть 2 случая (фиксируем $z$):
	$$0 \leq z \leq 1$$
	$$1 \leq z \leq \sqrt{2}$$  
	
	Тогда
	$$\int_0^1dz\left(\int_0^{\sqrt{z}}dx\int_{\sqrt{z-x^2}}^{1}f(x,y,z)dy + \int_{\sqrt{z}}^1dx\int_{0}^{1}f(x,y,z)dy\right) + \int_1^2dz\int_{\sqrt{z-1}}^1dx\int_{\sqrt{z-x^2}}^{1}f(x,y,z)dy$$
	\end{enumerate}
\end{document}